GenericModuleLib/SinglePassImplModule.v
@@ -1,0 +1,348 @@
+(* %%%%%%%%%%%%%%%%%%%%%%%%%%%%%%%%%%%%%%%%%%%%%%%%%%%%%%%%%%%%%%%%% *) 
+(* Module with Certified Checking 
+   of Single-Pass Implementation Module.
+  
+   Last Update: Fri, 26 May 2017
+ %%%%%%%%%%%%%%%%%%%%%%%%%%%%%%%%%%%%%%%%%%%%%%%%%%%%%%%%%%%%%%%%%%% *) 
+
+Add LoadPath "../..".
+
+Require Import ConceptParams.AuxTactics.LibTactics.
+Require Import ConceptParams.AuxTactics.BasicTactics.
+
+Require Import ConceptParams.SetMapLib.List2Set.
+Require Import ConceptParams.SetMapLib.ListPair2FMap.
+
+Require Import ConceptParams.GenericModuleLib.SharedDataDefs.
+
+Require Import Coq.Lists.List.
+Import ListNotations.
+Require Import Coq.Bool.Bool.
+
+Require Import Coq.Structures.Orders.
+Require Import Coq.Structures.Equalities.
+
+Require Import Coq.omega.Omega.
+
+(* ***************************************************************** *)
+(** * Single-Pass Implementation Module *)
+
+(** Single-Pass Module is well-defined if
+    all names are different 
+    and all members are well-defined with respect to some interface
+      with following elements
+      refering to the previously defined ones via local context. *)
+(* ***************************************************************** *)
+(* ***************************************************************** *)
+
+(* ################################################################# *)
+(** ** Shared Parameters of all building blocks *)
+(* ################################################################# *)
+
+Module Type SinglePassImplModuleBase.
+  Include ModuleBase.
+
+  Declare Module MD : DataLCI.
+  Import MD.
+
+  (** Initial local context *)
+  Parameter ctxl_init : ctxloc.
+  (** Update local context *)
+  Parameter upd_ctxloc : ctxloc -> ctx -> intrfs -> id -> t -> ctxloc.
+
+  (** Members which have to be defined by an interface *)
+  Parameter members_to_define : intrfs -> list id.
+End SinglePassImplModuleBase.
+
+(* ----------------------------------------------------------------- *)
+(** *** Aux Definitions (for implementation purposes only) *)
+(* ----------------------------------------------------------------- *)
+
+Module SinglePassImplModule_Data (Import MMB : SinglePassImplModuleBase) 
+<: GenericModule_Data. 
+
+  Definition dt := MD.t.
+  Definition ctx := (MD.ctx * MD.intrfs)%type.
+End SinglePassImplModule_Data.
+
+(* ################################################################# *)
+(** ** Propositional Part *)
+(* ################################################################# *)
+
+Module SinglePassImplModuleDefs (Import MMB : SinglePassImplModuleBase) 
+       (Import TOkD : DataLCIOkDef MMB.MId MMB.MD).
+
+  Module HelperD.
+    Export MMB.MD.
+    Definition dt := t.
+
+    (** We can use generic implementation of single-pass module
+        checking from the SharedDataDefs.
+        For this we need several aux functions. *)
+
+    Definition update_prop (ok : Prop) (ci : ctx * intrfs) 
+               (cl : ctxloc) (decl : id * dt) : Prop
+      := let (c, i) := ci in
+         let (nm, d) := decl in 
+         (* check curr member in the local context *)
+         TOkD.is_ok c i cl nm d  
+         (* and preserve previous members' part *)
+         /\ ok.
+
+    Definition update_ctxloc (cl : ctxloc) (ci : ctx * intrfs) 
+               (decl : id * dt) : ctxloc
+      := let (c, i) := ci in 
+         let (nm, d) := decl in 
+         upd_ctxloc cl c i nm d.
+
+    (** We can use generic implementation of module-welldefinedness *)
+    Module MData := SinglePassImplModule_Data MMB.
+    Module MSP := SinglePassModule_ProcessMembers.
+    Module MGM := GenericModule_ModuleOk MId.
+
+    (** Aux function checking that all members are ok. *)
+    Definition members_ok (ci : ctx * intrfs) 
+               (decls : list (id * dt)) : Prop 
+      := MSP.members_ok (ctx * intrfs) ctxloc (id * dt) 
+                        update_prop update_ctxloc ci ctxl_init decls.
+
+    Definition req_members_defined (i : intrfs) (decls : list (id * dt)) : Prop
+      := List.Forall 
+           (fun nm => List.In nm (map fst decls)) 
+           (members_to_define i).
+ 
+  End HelperD.
+  Import HelperD.
+
+  (** Single-Pass Module given as the AST [decls]  
+   ** is well-defined in the context [c]. *)
+  Definition module_ok (c : ctx) (i : intrfs) (decls : list (id * dt)) : Prop :=
+    MGM.module_ok MData.dt MData.ctx members_ok (c, i) decls
+    /\ (HelperD.req_members_defined i decls).
+
+End SinglePassImplModuleDefs.
+
+(* ################################################################# *)
+(** ** Computable Part (static checker of the interpreter) *)
+(* ################################################################# *)
+
+Module SinglePassImplModuleInterp (Import MMB : SinglePassImplModuleBase) 
+       (Import TOkI : DataLCIOkInterp MMB.MId MMB.MD).
+
+  Module HelperI.
+    Export MMB.MD.
+    Definition dt := t.
+
+    Definition check_member (ci : ctx * intrfs) 
+               (cl : ctxloc) (decl : id * dt) : bool
+      := let (c, i) := ci in 
+         let (nm, d) := decl in 
+         TOkI.is_ok_b c i cl nm d.
+
+    Definition update_ctxloc (cl : ctxloc) (ci : ctx * intrfs) 
+               (decl : id * dt) : ctxloc
+      := let (c, i) := ci in 
+         let (nm, d) := decl in 
+         upd_ctxloc cl c i nm d.
+
+    (** We can use generic implementation of module-welldefinedness *)
+    Module MData := SinglePassImplModule_Data MMB.
+    Module MSP := SinglePassModule_ProcessMembers.
+    Module MGM := GenericModule_ModuleOk MId.
+
+    (** Aux function checking that all members are ok. *)
+    Definition members_ok_b (ci : ctx * intrfs) 
+               (decls : list (id * dt)) : bool 
+      := MSP.members_ok_b (ctx * intrfs) ctxloc (id * dt)
+                          check_member update_ctxloc ci ctxl_init decls.
+
+    Definition req_members_defined_b (i : intrfs) (decls : list (id * dt)) : bool
+      := List.forallb 
+           (fun nm => Nat.leb 1 (List.count_occ MId.IdDT.eq_dec (map fst decls) nm)) 
+           (members_to_define i).
+
+  End HelperI.
+  Import HelperI.
+
+  (** Checks that a module given as the AST [decls]  
+   ** is well-defined in the context [c]. *)
+  Definition module_ok_b (c : ctx) (i : intrfs) 
+             (decls : list (id * dt)) : bool :=
+    andb 
+      (MGM.module_ok_b MData.dt MData.ctx members_ok_b (c, i) decls)
+      (req_members_defined_b i decls).
+
+End SinglePassImplModuleInterp.
+
+(* ################################################################# *)
+(** ** Proofs of Correctness *)
+(* ################################################################# *)
+
+Module SinglePassImplModuleProps 
+       (Import MMB : SinglePassImplModuleBase)
+       (Import TOkD : DataLCIOkDef MMB.MId MMB.MD)
+       (Import TOkI : DataLCIOkInterp MMB.MId MMB.MD)
+       (Import TOkP : DataLCIOkProp MMB.MId MMB.MD TOkD TOkI)
+.
+  Module Import MMD := SinglePassImplModuleDefs   MMB TOkD.
+  Module Import MMI := SinglePassImplModuleInterp MMB TOkI.
+  Import MMD.HelperD. Import MMI.HelperI.
+
+(* ----------------------------------------------------------------- *)
+(** *** Helper Props  *)
+(* ----------------------------------------------------------------- *)
+
+  Module Helper.
+    Import MMD.HelperD.
+ 
+    Lemma check_member__sound : 
+      forall (ci : ctx * intrfs) (cl : ctxloc) (decl : id * dt) (P : Prop),
+        P -> 
+        check_member ci cl decl = true ->
+        update_prop P ci cl decl.
+    Proof.
+      intros [c i] cl [nm d] P HP H.
+      unfold check_member in H. unfold update_prop.
+      apply TOkP.is_ok_b__sound in H. tauto.
+    Qed.
+
+    Lemma check_member__complete : 
+      forall (ci : ctx * intrfs) (cl : ctxloc) (decl : id * dt) (P : Prop),
+        P -> 
+        update_prop P ci cl decl ->
+        check_member ci cl decl = true.
+    Proof.
+      intros [c i] cl [nm d] P HP H.
+      unfold check_member. unfold update_prop in H.
+      apply TOkP.is_ok_b__complete. tauto.
+    Qed.
+
+    Lemma update_prop__spec :
+      forall (ci : ctx * intrfs) (cl : ctxloc) (decl : id * dt) (P : Prop),
+        update_prop P ci cl decl -> P.
+    Proof.
+      intros [c i] cl [nm d] P H.
+      unfold update_prop in H. tauto.
+    Qed.
+
+(* ----------------------------------------------------------------- *)
+    
+    (** We can use generic implementation of module-welldefinedness *)
+    Module MData := SinglePassImplModule_Data MMB.
+    Module MSP := SinglePassModule_ProcessMembers.
+    Module MGM := GenericModule_ModuleOk MId.
+
+    Lemma members_ok_b__sound :
+      forall (ci : ctx * intrfs) (decls : list (id * dt)),
+      members_ok_b ci decls = true ->
+      members_ok ci decls.
+    Proof.
+      intros ci ds H.
+      unfold members_ok_b in H.
+      unfold members_ok.
+      apply MSP.members_ok_b__sound with (update_prop := update_prop) in H.
+      assumption. 
+      exact check_member__sound.
+    Qed.
+
+    Lemma members_ok_b__complete :
+      forall (ci : ctx * intrfs) (decls : list (id * dt)),
+        members_ok ci decls -> 
+        members_ok_b ci decls = true.
+    Proof.
+      intros ci ds H.
+      unfold members_ok in H.
+      unfold members_ok_b.
+      apply MSP.members_ok_b__complete with (check_member := check_member) in H.
+      assumption. 
+      exact check_member__complete.
+      exact update_prop__spec.
+    Qed.
+
+(* ----------------------------------------------------------------- *) 
+
+    Lemma req_members_defined_b__sound :
+      forall (i : intrfs) (decls : list (id * dt)),
+        req_members_defined_b i decls = true ->
+        req_members_defined i decls.
+    Proof.
+      intros i.
+      unfold req_members_defined_b, req_members_defined.
+      induction (members_to_define i) as [| m ms IHms].
+      - (* no members to define *)
+        intros ds H. constructor.
+      - (* members_to_define = m :: ms *)
+        intros ds H.
+        simpl in *.
+        rewrite andb_true_iff in H. destruct H as [Hm Hms].
+        destruct (count_occ MId.IdDT.eq_dec (map fst ds) m) eqn:Heq.
+        rewrite Heq in Hm at 1.
+        inversion Hm. clear Hm.
+        constructor.
+        rewrite -> (count_occ_In MId.IdDT.eq_dec). omega.
+        apply IHms. assumption.
+    Qed.
+
+    Lemma req_members_defined_b__complete :
+      forall (i : intrfs) (decls : list (id * dt)),
+        req_members_defined i decls ->
+        req_members_defined_b i decls = true.
+    Proof.
+      intros i.
+      unfold req_members_defined_b, req_members_defined.
+      induction (members_to_define i) as [| m ms IHms].
+      - (* no members to define *)
+        intros ds H. simpl. reflexivity.
+      - (* members_to_define = m :: ms *)
+        intros ds H.
+        simpl in *.
+        rewrite andb_true_iff. 
+        inversion H as [Hm | Hms]; subst.
+        split.
+        + rewrite -> (count_occ_In MId.IdDT.eq_dec) in H0.
+          inversion H0. rewrite <- H3 at 1. reflexivity.
+          rewrite <- H2 at 1. reflexivity.
+        + specialize (IHms ds H1). assumption.
+    Qed.
+
+  End Helper.
+
+(* ================================================================= *)
+(** *** Properties *)
+(* ================================================================= *)
+
+  Theorem module_ok_b__sound : 
+    forall (c : ctx) (i : intrfs) (decls : list (id * dt)),
+      module_ok_b c i decls = true ->
+      module_ok c i decls.
+  Proof.
+    intros c i decls H.
+    unfold module_ok_b in H. unfold module_ok.
+    rewrite andb_true_iff in H. inversion H as [Hm Hids].
+    split.
+    - apply MGM.module_ok_b__sound 
+      with (members_ok := HelperD.members_ok) in Hm. assumption.
+      apply Helper.members_ok_b__sound.
+    - clear Hm.
+      apply Helper.req_members_defined_b__sound. assumption.
+  Qed.
+
+  Theorem module_ok_b__complete : 
+    forall (c : ctx) (i : intrfs) (decls : list (id * dt)),
+      module_ok c i decls ->
+      module_ok_b c i decls = true.
+  Proof.
+    intros c i decls H.
+    unfold module_ok in H. unfold module_ok_b.
+    rewrite andb_true_iff. inversion H as [Hm Hids].
+    split.
+    - apply MGM.module_ok_b__complete
+      with (members_ok := HelperD.members_ok); try assumption.
+      apply Helper.members_ok_b__complete.
+    - apply Helper.req_members_defined_b__complete; assumption.
+  Qed.
+
+End SinglePassImplModuleProps.
+
+
+
