Makefile
@@ -108,8 +108,6 @@ VFILES:=BasicPLDefs/Identifier.v\
   GenericModuleLib/SimpleModule.v\
   GenericModuleLib/SinglePassModule.v\
   GenericModuleLib/SinglePassImplModule.v\
-  GenericModuleLib/MIntrfs1.v\
-  GenericModuleLib/MImplmn1.v\
   cpSTLC/cpSTLCa_Defs.v\
   cpSTLC/cpSTLCa_Interpreter.v\
   cpSTLC/cpSTLCa_Examples.v\
